Convert `proof_checker` to `find_invalid_step`
The proof is invalid if there is an invalid step. With this API we can
easily point out which step is invalid, rather than saying the proof is
invalid without any further information.

bin/main.ml
@@ -9,15 +9,23 @@ let parse_proof _ =
 let parse_model _ =
   { Checker_extracted.constraints = []; Checker_extracted.variables = [] }
 
+(** Convert a `nat` extracted from Coq to an OCaml integer. *)
+let rec nat_to_int = function
+  | Checker_extracted.O -> 0
+  | Checker_extracted.S n -> 1 + nat_to_int n
+
 let check_proof model proof =
   if not (Sys.file_exists model) then `Error (false, model ^ ": not a file")
   else if not (Sys.file_exists proof) then `Error (false, proof ^ ": not a file")
   else
     let parsed_proof = parse_proof proof in
     let parsed_model = parse_model model in
-    if Checker_extracted.proof_checker parsed_proof parsed_model then
-      `Ok (print_endline "Proof is valid!")
-    else `Ok (print_endline "Proof is invalid!")
+    match Checker_extracted.find_invalid_step parsed_proof parsed_model with
+    | Some (step_nr, _) ->
+        `Ok
+          (Printf.printf "Proof is invalid! Rejected proof step %d\n"
+             (nat_to_int step_nr))
+    | None -> `Ok (print_endline "Proof is valid!")
 
 let model_t =
   let doc = "The FZN file describing the model." in
