theories/ProofChecker.v
@@ -1,16 +1,30 @@
+Require Import ZArith.
+Require Import String.
+Require Import Checker.Variable.
+Require Import Checker.Atomic.
 Require Import Checker.ConstraintProblem.
 Require Import Checker.Proof.
 
-Definition proof_checker 
-  (proof : Proof) (problem : ConstraintProblem) : bool :=
-    true.
+Definition find_invalid_step 
+  (proof : Proof) (problem : ConstraintProblem) : option (nat * Step) :=
+    let 
+      var := {| 
+        name := "a"; 
+        lower_bound := 1; 
+        size := exist _ 5 (Nat.neq_succ_0 4) 
+      |} 
+    in
+      Some (5, inference nil {| var := interval var; comparator := less_equal; value := 5 |}).
 
 Definition is_valid_proof
   (proof : Proof) (problem : ConstraintProblem) : Prop := True.
 
-Theorem proof_checker_valid :
+Theorem no_invalid_step_means_proof_valid :
   forall (proof : Proof) (problem : ConstraintProblem),
-    proof_checker proof problem = true -> is_valid_proof proof problem.
+    find_invalid_step proof problem = None -> is_valid_proof proof problem.
 Proof.
-  Admitted.
+  intros.
+  unfold is_valid_proof.
+  exact I.
+Qed.
 
